theories/Numbers/Rational/BigQ/QMake.v
@@ -57,7 +57,7 @@ Module Make (N:NType)(Z:ZType)(Import NZ:NType_ZType N Z) <: QType.
  Definition to_Q (q: t) :=
  match q with
    | Qz x => Z.to_Z x # 1
-   | Qq x y => if N.eq_bool y N.zero then 0
+   | Qq x y => if N.eqb y N.zero then 0
                else Z.to_Z x # Z2P (N.to_Z y)
  end.
 
@@ -79,15 +79,13 @@ Module Make (N:NType)(Z:ZType)(Import NZ:NType_ZType N Z) <: QType.
 *)
  Ltac destr_eqb :=
   match goal with
-   | |- context [Z.eq_bool ?x ?y] =>
-     rewrite (Z.spec_eq_bool x y);
-     generalize (Zeq_bool_if (Z.to_Z x) (Z.to_Z y));
-     case (Zeq_bool (Z.to_Z x) (Z.to_Z y));
+   | |- context [Z.eqb ?x ?y] =>
+     rewrite (Z.spec_eqb x y);
+     case (Z.eqb_spec (Z.to_Z x) (Z.to_Z y));
      destr_eqb
-   | |- context [N.eq_bool ?x ?y] =>
-     rewrite (N.spec_eq_bool x y);
-     generalize (Zeq_bool_if (N.to_Z x) (N.to_Z y));
-     case (Zeq_bool (N.to_Z x) (N.to_Z y));
+   | |- context [N.eqb ?x ?y] =>
+     rewrite (N.spec_eqb x y);
+     case (Z.eqb_spec (N.to_Z x) (N.to_Z y));
      [ | let H:=fresh "H" in
          try (intro H;generalize (N_to_Z_pos _ H); clear H)];
      destr_eqb
@@ -145,13 +143,13 @@ Module Make (N:NType)(Z:ZType)(Import NZ:NType_ZType N Z) <: QType.
   match x, y with
   | Qz zx, Qz zy => Z.compare zx zy
   | Qz zx, Qq ny dy =>
-    if N.eq_bool dy N.zero then Z.compare zx Z.zero
+    if N.eqb dy N.zero then Z.compare zx Z.zero
     else Z.compare (Z.mul zx (Z_of_N dy)) ny
   | Qq nx dx, Qz zy =>
-    if N.eq_bool dx N.zero then Z.compare Z.zero zy
+    if N.eqb dx N.zero then Z.compare Z.zero zy
     else Z.compare nx (Z.mul zy (Z_of_N dx))
   | Qq nx dx, Qq ny dy =>
-    match N.eq_bool dx N.zero, N.eq_bool dy N.zero with
+    match N.eqb dx N.zero, N.eqb dy N.zero with
     | true, true => Eq
     | true, false => Z.compare Z.zero ny
     | false, true => Z.compare nx Z.zero
@@ -301,15 +299,15 @@ Module Make (N:NType)(Z:ZType)(Import NZ:NType_ZType N Z) <: QType.
     match y with
     | Qz zy => Qz (Z.add zx zy)
     | Qq ny dy =>
-      if N.eq_bool dy N.zero then x
+      if N.eqb dy N.zero then x
       else Qq (Z.add (Z.mul zx (Z_of_N dy)) ny) dy
     end
   | Qq nx dx =>
-    if N.eq_bool dx N.zero then y
+    if N.eqb dx N.zero then y
     else match y with
     | Qz zy => Qq (Z.add nx (Z.mul zy (Z_of_N dx))) dx
     | Qq ny dy =>
-      if N.eq_bool dy N.zero then x
+      if N.eqb dy N.zero then x
       else
        let n := Z.add (Z.mul nx (Z_of_N dy)) (Z.mul ny (Z_of_N dx)) in
        let d := N.mul dx dy in
@@ -333,15 +331,15 @@ Module Make (N:NType)(Z:ZType)(Import NZ:NType_ZType N Z) <: QType.
     match y with
     | Qz zy => Qz (Z.add zx zy)
     | Qq ny dy =>
-      if N.eq_bool dy N.zero then x
+      if N.eqb dy N.zero then x
       else norm (Z.add (Z.mul zx (Z_of_N dy)) ny) dy
     end
   | Qq nx dx =>
-    if N.eq_bool dx N.zero then y
+    if N.eqb dx N.zero then y
     else match y with
     | Qz zy => norm (Z.add nx (Z.mul zy (Z_of_N dx))) dx
     | Qq ny dy =>
-      if N.eq_bool dy N.zero then x
+      if N.eqb dy N.zero then x
       else
        let n := Z.add (Z.mul nx (Z_of_N dy)) (Z.mul ny (Z_of_N dx)) in
        let d := N.mul dx dy in
@@ -378,8 +376,8 @@ Module Make (N:NType)(Z:ZType)(Import NZ:NType_ZType N Z) <: QType.
  Proof.
  intros [z | x y]; simpl.
  rewrite Z.spec_opp; auto.
- match goal with  |- context[N.eq_bool ?X ?Y] =>
-  generalize (N.spec_eq_bool X Y); case N.eq_bool
+ match goal with  |- context[N.eqb ?X ?Y] =>
+  generalize (N.spec_eqb X Y); case N.eqb
  end; auto; rewrite N.spec_0.
  rewrite Z.spec_opp; auto.
  Qed.
@@ -429,26 +427,29 @@ Module Make (N:NType)(Z:ZType)(Import NZ:NType_ZType N Z) <: QType.
   | Qq nx dx, Qq ny dy => Qq (Z.mul nx ny) (N.mul dx dy)
   end.
 
+ Ltac nsubst :=
+  match goal with E : N.to_Z _ = _ |- _ => rewrite E in * end.
+
  Theorem spec_mul : forall x y, [mul x y] == [x] * [y].
  Proof.
  intros [x | nx dx] [y | ny dy]; unfold Qmult; simpl; qsimpl.
  rewrite Pmult_1_r, Z2P_correct; auto.
  destruct (Zmult_integral (N.to_Z dx) (N.to_Z dy)); intuition.
- rewrite H0 in H1; auto with zarith.
- rewrite H0 in H1; auto with zarith.
- rewrite H in H1; nzsimpl; auto with zarith.
+ nsubst; auto with zarith.
+ nsubst; auto with zarith.
+ nsubst; nzsimpl; auto with zarith.
  rewrite Zpos_mult_morphism, 2 Z2P_correct; auto.
  Qed.
 
  Definition norm_denum n d :=
-  if N.eq_bool d N.one then Qz n else Qq n d.
+  if N.eqb d N.one then Qz n else Qq n d.
 
  Lemma spec_norm_denum : forall n d,
   [norm_denum n d] == [Qq n d].
  Proof.
  unfold norm_denum; intros; simpl; qsimpl.
  congruence.
- rewrite H0 in *; auto with zarith.
+ nsubst; auto with zarith.
  Qed.
 
  Definition irred n d :=
@@ -528,7 +529,7 @@ Module Make (N:NType)(Z:ZType)(Import NZ:NType_ZType N Z) <: QType.
  Qed.
 
  Definition mul_norm_Qz_Qq z n d :=
-   if Z.eq_bool z Z.zero then zero
+   if Z.eqb z Z.zero then zero
    else
     let gcd := N.gcd (Zabs_N z) d in
     match N.compare gcd N.one with
@@ -561,7 +562,7 @@ Module Make (N:NType)(Z:ZType)(Import NZ:NType_ZType N Z) <: QType.
  rewrite spec_norm_denum.
  qsimpl.
  rewrite Zdiv_gcd_zero in GT; auto with zarith.
- rewrite H in *. rewrite Zdiv_0_l in *; discriminate.
+ nsubst. rewrite Zdiv_0_l in *; discriminate.
  rewrite <- Zmult_assoc, (Zmult_comm (Z.to_Z n)), Zmult_assoc.
  rewrite Zgcd_div_swap0; try romega.
  ring.
@@ -637,13 +638,15 @@ Module Make (N:NType)(Z:ZType)(Import NZ:NType_ZType N Z) <: QType.
  rewrite spec_norm_denum.
  qsimpl.
 
- destruct (Zmult_integral _ _ H0) as [Eq|Eq].
+ match goal with E : (_ * _ = 0)%Z |- _ =>
+  destruct (Zmult_integral _ _ E) as [Eq|Eq] end.
  rewrite Eq in *; simpl in *.
  rewrite <- Hg2' in *; auto with zarith.
  rewrite Eq in *; simpl in *.
  rewrite <- Hg2 in *; auto with zarith.
 
- destruct (Zmult_integral _ _ H) as [Eq|Eq].
+ match goal with E : (_ * _ = 0)%Z |- _ =>
+  destruct (Zmult_integral _ _ E) as [Eq|Eq] end.
  rewrite Hz' in Eq; rewrite Eq in *; auto with zarith.
  rewrite Hz in Eq; rewrite Eq in *; auto with zarith.
 
@@ -691,13 +694,13 @@ Module Make (N:NType)(Z:ZType)(Import NZ:NType_ZType N Z) <: QType.
 
  rewrite Zgcd_1_rel_prime in *.
  apply bezout_rel_prime.
- destruct (rel_prime_bezout _ _ H4) as [u v Huv].
+ destruct (rel_prime_bezout (Z.to_Z ny) (N.to_Z dy)) as [u v Huv]; trivial.
  apply Bezout_intro with (u*g')%Z (v*g)%Z.
  rewrite <- Huv, <- Hg1', <- Hg2. ring.
 
  rewrite Zgcd_1_rel_prime in *.
  apply bezout_rel_prime.
- destruct (rel_prime_bezout _ _ H3) as [u v Huv].
+ destruct (rel_prime_bezout (Z.to_Z nx) (N.to_Z dx)) as [u v Huv]; trivial.
  apply Bezout_intro with (u*g)%Z (v*g')%Z.
  rewrite <- Huv, <- Hg2', <- Hg1. ring.
  Qed.
@@ -755,10 +758,7 @@ Module Make (N:NType)(Z:ZType)(Import NZ:NType_ZType N Z) <: QType.
  destr_eqb; nzsimpl; intros.
  intros; rewrite Zabs_eq in *; romega.
  intros; rewrite Zabs_eq in *; romega.
- clear H1.
- rewrite H0.
- compute; auto.
- clear H1.
+ nsubst; compute; auto.
  set (n':=Z.to_Z n) in *; clearbody n'.
  rewrite Zabs_eq by romega.
  red; simpl.
@@ -770,9 +770,7 @@ Module Make (N:NType)(Z:ZType)(Import NZ:NType_ZType N Z) <: QType.
  destr_eqb; nzsimpl; intros.
  intros; rewrite Zabs_non_eq in *; romega.
  intros; rewrite Zabs_non_eq in *; romega.
- clear H1.
- red; nzsimpl; rewrite H0; compute; auto.
- clear H1.
+ nsubst; compute; auto.
  set (n':=Z.to_Z n) in *; clearbody n'.
  red; simpl; nzsimpl.
  rewrite Zabs_non_eq by romega.
@@ -791,7 +789,7 @@ Module Make (N:NType)(Z:ZType)(Import NZ:NType_ZType N Z) <: QType.
          | Gt => Qq Z.minus_one (Zabs_N z)
        end
      | Qq n d =>
-       if N.eq_bool d N.zero then zero else
+       if N.eqb d N.zero then zero else
        match Z.compare Z.zero n with
          | Eq => zero
          | Lt =>
@@ -928,9 +926,9 @@ Module Make (N:NType)(Z:ZType)(Import NZ:NType_ZType N Z) <: QType.
  destr_eqb; nzsimpl; intros.
  apply Qeq_refl.
  rewrite N.spec_square in *; nzsimpl.
- elim (Zmult_integral _ _ H0); romega.
- rewrite N.spec_square in *; nzsimpl.
- rewrite H in H0; romega.
+ match goal with E : (_ * _ = 0)%Z |- _ =>
+  elim (Zmult_integral _ _ E); romega end.
+ rewrite N.spec_square in *; nzsimpl; nsubst; romega.
  rewrite Z.spec_square, N.spec_square.
  red; simpl.
  rewrite Zpos_mult_morphism; rewrite !Z2P_correct; auto.
@@ -961,8 +959,9 @@ Module Make (N:NType)(Z:ZType)(Import NZ:NType_ZType N Z) <: QType.
  assert (0 < N.to_Z d ^ ' p)%Z by
   (apply Zpower_gt_0; auto with zarith).
  romega.
- rewrite N.spec_pow_pos, H in *.
- rewrite Zpower_0_l in H0; [romega|discriminate].
+ exfalso.
+ rewrite N.spec_pow_pos in *. nsubst.
+ rewrite Zpower_0_l in *; [romega|discriminate].
  rewrite Qpower_decomp.
  red; simpl; do 3 f_equal.
  rewrite Z2P_correct by (generalize (N.spec_pos d); romega).
@@ -981,8 +980,9 @@ Module Make (N:NType)(Z:ZType)(Import NZ:NType_ZType N Z) <: QType.
  revert H.
  unfold Reduced; rewrite strong_spec_red, Qred_iff; simpl.
  destr_eqb; nzsimpl; simpl; intros.
- rewrite N.spec_pow_pos in H0.
- rewrite H, Zpower_0_l in *; [romega|discriminate].
+ exfalso.
+ rewrite N.spec_pow_pos in *. nsubst.
+ rewrite Zpower_0_l in *; [romega|discriminate].
  rewrite Z2P_correct in *; auto.
  rewrite N.spec_pow_pos, Z.spec_pow_pos; auto.
  rewrite Zgcd_1_rel_prime in *.
