theories/Structures/Equalities.v
@@ -66,10 +66,19 @@ End HasEqDec.
 (** Having [eq_dec] is the same as having a boolean equality plus
     a correctness proof. *)
 
-Module Type HasEqBool (Import E:Eq').
+Module Type HasEqb (Import T:Typ).
   Parameter Inline eqb : t -> t -> bool.
-  Parameter eqb_eq : forall x y, eqb x y = true <-> x==y.
-End HasEqBool.
+End HasEqb.
+
+Module Type EqbSpec (T:Typ)(X:HasEq T)(Y:HasEqb T).
+  Parameter eqb_eq : forall x y, Y.eqb x y = true <-> X.eq x y.
+End EqbSpec.
+
+Module Type EqbNotation (T:Typ)(E:HasEqb T).
+  Infix "=?" := E.eqb (at level 70, no associativity).
+End EqbNotation.
+
+Module Type HasEqBool (E:Eq) := HasEqb E <+ EqbSpec E E.
 
 (** From these basic blocks, we can build many combinations
     of static standalone module types. *)
@@ -107,8 +116,10 @@ Module Type EqualityTypeBoth' := EqualityTypeBoth <+ EqNotation.
 Module Type DecidableType' := DecidableType <+ EqNotation.
 Module Type DecidableTypeOrig' := DecidableTypeOrig <+ EqNotation.
 Module Type DecidableTypeBoth' := DecidableTypeBoth <+ EqNotation.
-Module Type BooleanEqualityType' := BooleanEqualityType <+ EqNotation.
-Module Type BooleanDecidableType' := BooleanDecidableType <+ EqNotation.
+Module Type BooleanEqualityType' :=
+ BooleanEqualityType <+ EqNotation <+ EqbNotation.
+Module Type BooleanDecidableType' :=
+ BooleanDecidableType <+ EqNotation <+ EqbNotation.
 Module Type DecidableTypeFull' := DecidableTypeFull <+ EqNotation.
 
 (** * Compatibility wrapper from/to the old version of
@@ -166,9 +177,12 @@ Module Dec2Bool (E:DecidableType) <: BooleanDecidableType
 Module Bool2Dec (E:BooleanEqualityType) <: BooleanDecidableType
  := E <+ HasEqBool2Dec.
 
-(** In a BooleanEqualityType, [eqb] is compatible with [eq] *)
 
-Module BoolEqualityFacts (Import E : BooleanEqualityType).
+(** Some properties of boolean equality *)
+
+Module BoolEqualityFacts (Import E : BooleanEqualityType').
+
+(** [eqb] is compatible with [eq] *)
 
 Instance eqb_compat : Proper (E.eq ==> E.eq ==> Logic.eq) eqb.
 Proof.
@@ -176,6 +190,34 @@ intros x x' Exx' y y' Eyy'.
 apply eq_true_iff_eq.
 now rewrite 2 eqb_eq, Exx', Eyy'.
 Qed.
+
+(** Alternative specification of [eqb] based on [reflect]. *)
+
+Lemma eqb_spec x y : reflect (x==y) (x =? y).
+Proof.
+apply iff_reflect. symmetry. apply eqb_eq.
+Qed.
+
+(** Negated form of [eqb_eq] *)
+
+Lemma eqb_neq x y : (x =? y) = false <-> x ~= y.
+Proof.
+now rewrite <- not_true_iff_false, eqb_eq.
+Qed.
+
+(** Basic equality laws for [eqb] *)
+
+Lemma eqb_refl x : (x =? x) = true.
+Proof.
+now apply eqb_eq.
+Qed.
+
+Lemma eqb_sym x y : (x =? y) = (y =? x).
+Proof.
+apply eq_true_iff_eq. now rewrite 2 eqb_eq.
+Qed.
+
+(** Transitivity is a particular case of [eqb_compat] *)
 
 End BoolEqualityFacts.
 
